Refactored STMDefs into several files
Also got extraction almost working, except for some extraneous
typeclasses

tests/monadic/stm/stm.cpp
@@ -1,74 +1,53 @@
 #include "stm.h"
 
-uint64_t stmtest::stm_basic_counter(std::monostate) {
-  stm::TVar<uint64_t> c = stm::newTVar(UINT64_C(0));
-  stm::writeTVar(c, UINT64_C(1));
-  return stm::readTVar(std::move(c));
+uint64_t stmtest::basic_read(uint64_t x) {
+  stm::TVar<uint64_t> c = stm::atomically([&] { return stm::newTVar(x); });
+  return stm::atomically([&] { return stm::readTVar(c); });
 }
 
-uint64_t stmtest::io_basic_counter() {
-  return stm::atomically([&] { return stm_basic_counter(std::monostate{}); });
+uint64_t stmtest::basic_write(uint64_t x) {
+  stm::TVar<uint64_t> c =
+      stm::atomically([&] { return stm::newTVar(UINT64_C(0)); });
+  stm::atomically([&] {
+    return [&]() {
+      stm::writeTVar(c, x);
+      return std::monostate{};
+    }();
+  });
+  return stm::atomically([&] { return stm::readTVar(c); });
 }
 
-uint64_t stmtest::stm_inc(uint64_t x) {
-  stm::TVar<uint64_t> c = stm::newTVar(x);
-  STMDefs::template modifyTVar<uint64_t>(c, [](uint64_t n) { return (n + 1); });
-  return stm::readTVar(std::move(c));
+uint64_t stmtest::increment(uint64_t x) {
+  stm::TVar<uint64_t> c = stm::atomically([&] { return stm::newTVar(x); });
+  stm::atomically([&] {
+    return [&]() {
+      STMDefs::modifyTVar(c, [](uint64_t x0) { return (x0 + 1); });
+      return std::monostate{};
+    }();
+  });
+  return stm::atomically([&] { return stm::readTVar(c); });
 }
 
-uint64_t stmtest::io_inc(uint64_t x) {
-  return stm::atomically([&] { return stm_inc(x); });
+uint64_t stmtest::write_read(uint64_t x) {
+  stm::TVar<uint64_t> c =
+      stm::atomically([&] { return stm::newTVar(UINT64_C(0)); });
+  return stm::atomically([&] {
+    return [=]() mutable {
+      stm::writeTVar(c, x);
+      return stm::readTVar(c);
+    }();
+  });
 }
 
-uint64_t stmtest::stm_add_self(uint64_t x) {
-  stm::TVar<uint64_t> c = stm::newTVar(x);
-  uint64_t v = stm::readTVar(c);
-  stm::writeTVar(c, (v + x));
-  return stm::readTVar(std::move(c));
-}
-
-uint64_t stmtest::io_add_self(uint64_t x) {
-  return stm::atomically([&] { return stm_add_self(x); });
-}
-
-void stmtest::stm_enqueue(stm::TVar<List<uint64_t>> q, uint64_t x) {
-  List<uint64_t> xs = stm::readTVar(q);
-  stm::writeTVar(
-      q, std::move(xs).app(List<uint64_t>::cons(x, List<uint64_t>::nil())));
-  return;
-}
-
-uint64_t stmtest::stm_dequeue(stm::TVar<List<uint64_t>> q) {
-  List<uint64_t> xs = stm::readTVar(q);
-  if (std::holds_alternative<typename List<uint64_t>::Nil>(xs.v_mut())) {
-    return stm::retry<uint64_t>();
-  } else {
-    auto &[a0, a1] = std::get<typename List<uint64_t>::Cons>(xs.v_mut());
-    stm::writeTVar(q, *a1);
-    return a0;
-  }
-}
-
-uint64_t stmtest::stm_tryDequeue(stm::TVar<List<uint64_t>> q, uint64_t dflt) {
-  return stm::orElse<uint64_t>(stm_dequeue(q), dflt);
-}
-
-uint64_t stmtest::stm_queue_roundtrip(uint64_t x) {
-  stm::TVar<List<uint64_t>> q = stm::newTVar(List<uint64_t>::nil());
-  stm_enqueue(q, x);
-  return stm_dequeue(std::move(q));
-}
-
-uint64_t stmtest::io_queue_roundtrip(uint64_t x) {
-  return stm::atomically([&] { return stm_queue_roundtrip(x); });
-}
-
-uint64_t stmtest::stm_orElse_retry_example(std::monostate) {
-  stm::TVar<List<uint64_t>> q = stm::newTVar(List<uint64_t>::nil());
-  return stm::orElse<uint64_t>(stm_dequeue(std::move(q)), UINT64_C(42));
-}
-
-uint64_t stmtest::io_orElse_retry_example() {
-  return stm::atomically(
-      [&] { return stm_orElse_retry_example(std::monostate{}); });
+uint64_t stmtest::io_queue_roundtrip(uint64_t x, uint64_t y) {
+  stm::TVar<List<uint64_t>> q =
+      stm::atomically([&] { return stm::newTVar(List<uint64_t>::nil()); });
+  stm::atomically([&] {
+    return [&]() {
+      stm_enqueue(q, x);
+      stm_enqueue(q, y);
+      return std::monostate{};
+    }();
+  });
+  return stm::atomically([&] { return stm_dequeue(q); });
 }
