tests/monadic/stm/stm.t.cpp
@@ -34,7 +34,7 @@ void aSsErT(bool condition, const char *message, int line) {
 #define ASSERT(X) aSsErT(!(X), #X, __LINE__);
 
 int main() {
-  auto x = stmtest::io_inc(4);
+  auto x = stmtest::increment(4);
   std::cout << std::to_string(x) << '\n';
   // auto p = io_transfer_test(23, 32, 8);
   // std::cout << p.first << ", " << p.second << '\n';
