theories/Monads/STMDefs.v
@@ -8,34 +8,11 @@
    identical across library flavors. Flavor files ([STM.v], [STMBDE.v])
    re-export this module and add flavor-specific C++ extraction mappings.
 *)
-From Corelib Require Import PrimString PrimInt63.
+From Corelib Require Import PrimString.
 From Crane Require Extraction.
-From Crane Require Import Monads.ITree Monads.IODefs External.VectorDefs Utils.HMap Utils.HAList.
+From Crane Require Import Monads.ITree.
 
-
-
-From ITree Require Import
-  Basics.Basics
-  Basics.CategoryOps
-  Basics.CategoryKleisli
-  Core.Subevent
-  Events.FailFacts
-  Events.State
-  Indexed.Function
-  Indexed.Sum
-  Interp.Interp.
-
-
-
-Import Basics.Monads.
-
-From ExtLib Require Import Data.List Structures.Monad Structures.Reducible.
-
-From Stdlib Require Import List Classes.EquivDec Arith.PeanoNat Bool.Bool.
-
-From Crane Require Import Mergesort.
-
-Import ListNotations.
+From ITree Require Import Basics.Basics.
 
 Open Scope itree_scope.
 
@@ -60,47 +37,22 @@ Arguments WriteTVar {K} {V} {A}.
 Inductive stmControlE : Type -> Type :=
 | Retry : stmControlE void.
 
-Definition retry {E} `{stmControlE -< E} {A} : itree E A :=
-  trigger Retry >>= fun (x : void) => match x with end.
-
 Crane Extract Inductive stmControlE => ""
-  [ "stm::retry<%t0>()" ].
+  [ "stm::retry()" ].
 
 Definition stmE {K} (V : K -> Type) : Type -> Type := stmControlE +' tvarE V.
 Crane Extract Skip stmE.
 
+Definition retry {K} {V : K -> Type} {A} : itree (stmE V) A :=
+  trigger (inl1 Retry) >>= fun (x : void) => match x with end.
+
 (* not entirely sure why this is required *)
+(*
 #[global] Instance tvarE_sub_stmE {K} (V : K -> Type) : tvarE V -< stmE V := inr1.
 #[global] Instance stmControlE_sub_stmE {K} (V : K -> Type) : stmControlE -< stmE V := inl1.
-
-
-
-Definition pkey (K J : Type) := (K * J)%type.
-Definition pkey_type {K J} (V : K -> Type) (pk : pkey K J) := V (fst pk).
-
-Definition commit_log {K} (V : K -> Type) {M} `{Foldable M (sigT (pkey_type V))} {E} `{H : tvarE V -< E} : M -> itree E unit :=
-  fold (fun '(existT _ (k, n) v) acc => Vis (subevent (H := H) _ (WriteTVar (mk_tvar V n k) v)) (fun _ => acc)) (Ret tt).
-
-Definition handle_tvar_log {K} {V : K -> Type} {M} `{HMap (pkey K nat) (pkey_type V) M} {E} `{H : tvarE V -< E}
-  (m : M) : forall {A}, tvarE V A -> itree E (A * M) :=
-  fun _ t =>
-    match t with
-    | NewTVar k v => Vis (subevent (H := H) _ (NewTVar k v)) (fun tv => Ret (tv, m))
-    | ReadTVar tv =>
-        (let '(mk_tvar _ n k) in TVar _ T := tv return TVar V T -> itree E (T * M) in
-          match lookup (k, n) m with
-          | Some v => fun _ => Ret (v, m)
-          | None => fun tv => Vis (subevent (H := H) _ (ReadTVar tv)) (fun v => Ret (v, m))
-          end) tv
-    | WriteTVar (mk_tvar _ n k) v => Ret (tt, add (k, n) v m)
-    end.
-
-
-
-Variant atomicE E : Type -> Type :=
-| Atomic : forall {A} (t : itree E A), atomicE E A.
-
-Arguments Atomic {E} {A} (_).
+Crane Extract Skip tvarE_sub_stmE.
+Crane Extract Skip stmControlE_sub_stmE.
+*)
 
 
 
@@ -112,57 +64,13 @@ Arguments Atomically {K} {V} {A} (t).
 Definition atomically {K} {V : K -> Type} {E} `{runStmE V -< E} {A} (t : itree (stmE V) A) : itree E A :=
   trigger (Atomically t).
 
-
-
-Variant transactionE E : Type -> Type :=
-| Transaction : forall {A}, itree E A -> transactionE E (option A).
-
-Arguments Transaction {E} {A} (_).
+Crane Extract Inductive runStmE => ""
+  [ "stm::atomically([&] { return %a0; })" ].
 
 
 
-Definition h_atomically {K} {V : K -> Type} {E} `{transactionE (stmE V) -< E} : runStmE V ~> itree E :=
-  fun _ e =>
-    match e with
-    | Atomically t =>
-        ITree.iter (fun _ =>
-                      oa <- trigger (Transaction t) ;;
-                      match oa with
-                      | None => Ret (inl tt)
-                      | Some a => Ret (inr a)
-                      end) tt
-    end.
-
-
-
-Definition h_stm_write_log {K} {V : K -> Type} {M} `{HMap (pkey K nat) (pkey_type V) M} {E} `{tvarE V -< E}:
-  stmE V ~> stateT M (failT (itree E)) :=
-  fun _ e m =>
-    match e with
-    | inl1 Retry => Ret None
-    | inr1 e =>
-        '(a, m) <- handle_tvar_log m e ;;
-        Ret (Some (m, a))
-    end.
-
-(* TODO: generalize to any HMap *)
-(* Implements transactions by executing them atomically (blocks all other threads from executing until it is finished) *)
-Definition atomic_transactions {K} {V : K -> Type} `{EqDec K eq}: transactionE (stmE V) ~> atomicE (tvarE V) :=
-  fun _ e =>
-    match e with
-    | Transaction t =>
-        let m : stateT (halist (pkey K nat) (pkey_type V)) (failT (itree (tvarE V))) _ :=
-          interp h_stm_write_log t in
-        Atomic (res <- m [] ;;
-                match res with
-                | Some (m, a) =>
-                    commit_log _ m ;;
-                    Ret (Some a)
-                | None => Ret None
-                end)
-    end.
-
-Definition orElse {A} {K} {V : K -> Type} `{EqDec K eq} (t1 t2 : itree (stmE V) A) : itree (stmE V) A :=
+(*
+Definition orElse {A} {K} {V : K -> Type} `{EqDec K eq} (t1 t2 : itree (stmControlE +' tvarE V) A) : itree (stmE V) A :=
   (cofix _orElse (m : halist (pkey K nat) (pkey_type V)) t :=
     match observe t with
     | RetF a =>
@@ -172,365 +80,13 @@ Definition orElse {A} {K} {V : K -> Type} `{EqDec K eq} (t1 t2 : itree (stmE V) 
     | VisF (inr1 e) k => '(x, m) <- handle_tvar_log m e ;; Tau (_orElse m (k x))
     | VisF (inl1 Retry) _ => t2
     end) HMap.empty t1.
+*)
 
 
 
-Variant lockE : Type -> Type :=
-| TryLock : lockE bool
-| Unlock : lockE unit.
-
-Definition spinlock {E} `{lockE -< E} : itree E unit :=
-  ITree.iter (fun n => b <- trigger TryLock ;; if (b : bool) then Ret (inr tt) else Ret (inl (S n))) 0.
-
-(* TODO: generalize to any HMap *)
-(* implements transactions through a single global lock that is acquired before transaction execution *)
-Definition single_global_lock {K} {V : K -> Type} `{EqDec K eq} {E} `{lockE -< E} `{tvarE V -< E}:
-  transactionE (stmE V) ~> itree E :=
-  fun _ e =>
-    match e with
-    | Transaction t =>
-        spinlock ;;
-        let m : stateT (halist (pkey K nat) (pkey_type V)) (failT (itree E)) _ :=
-          interp h_stm_write_log t in
-        res <- m [] ;;
-        match res with
-        | Some (m, a) =>
-            commit_log _ m ;;
-            trigger Unlock ;;
-            Ret (Some a)
-        | None =>
-            trigger Unlock ;;
-            Ret None
-        end
-    end.
-
-Definition h_lock {E} : lockE ~> stateT bool (itree E) :=
-  fun _ e l =>
-    match e with
-    | TryLock => Ret (true, negb l)
-    | Unlock => Ret (false, tt)
-    end.
-
-
-
-
-Variant tl2E {K} (V : K -> Type) : Type -> Type :=
-| GetVersionClock : tl2E V nat
-| IncVersionClock : tl2E V nat
-| NewTVarTL2 : forall (k : K), V k -> tl2E V (TVar V (V k))
-| ReadTVarTL2 : forall {A}, TVar V A -> tl2E V (A * nat * bool)
-| WriteTVarTL2 : forall {A}, TVar V A -> A -> nat -> bool -> tl2E V unit
-| TryLockTVar : forall {A}, TVar V A -> tl2E V bool
-| UnlockTVar : forall {A}, TVar V A -> tl2E V unit.
-
-Arguments GetVersionClock {K} {V}.
-Arguments IncVersionClock {K} {V}.
-Arguments NewTVarTL2 {K} {V} (_ _).
-Arguments ReadTVarTL2 {K} {V} {A} (_).
-Arguments WriteTVarTL2 {K} {V} {A} (_ _ _ _).
-Arguments TryLockTVar {K} {V} {A} (_).
-Arguments UnlockTVar {K} {V} {A} (_).
-
-
-
-(* a blocking spinlock *)
-Definition spinlock_tvar {K} {V : K -> Type} {E} `{tl2E V -< E} {A} (x : TVar V A) : itree E unit :=
-  ITree.iter (fun _ => b <- trigger (TryLockTVar x) ;; if (b : bool) then Ret (inr tt) else Ret (inl tt)) tt.
-
-
-
-Variant errorE : Type -> Type :=
-| Error (msg : string) : errorE void.
-
-Definition error {E A} `{errorE -< E} (msg : string) : itree E A :=
-  Vis (subevent _ (Error msg)) (fun (x : void) => match x with end).
-
-
-
-Definition handle_tvar_log_tl2 {K} {V : K -> Type} {M} `{HMap (pkey K nat) (pkey_type V) M} {E} `{H : tl2E V -< E}
-  (rv : nat) : stmE V ~> stateT (list (pkey K nat) * M) (failT (itree E)) :=
-  fun _ t '(s_r, m_w) =>
-    match t with
-    | inl1 Retry => Ret None
-    | inr1 e =>
-      match e with
-      | NewTVar k v => Vis (subevent (H := H) _ (NewTVarTL2 k v)) (fun tv => Ret (Some ((s_r, m_w), tv)))
-      | ReadTVar tv =>
-          (let '(mk_tvar _ n k) in TVar _ T := tv return TVar V T -> itree E (option ((list (pkey K nat) * M) * T)) in
-            match lookup (k, n) m_w with
-            | Some v => fun _ => Ret (Some ((s_r, m_w), v))
-            | None => fun tv =>
-                '(v, ver, l) <- Vis (subevent (H := H) _ (ReadTVarTL2 tv)) (fun x => Ret x);;
-                if l || (rv <? ver)
-                then Ret None
-                else Ret (Some (((k, n) :: s_r, m_w), v))
-            end) tv
-      | WriteTVar (mk_tvar _ n k) v => Ret (Some ((s_r, add (k, n) v m_w), tt))
-      end
-    end.
-
-Definition write_tl2 {K} (V : K -> Type) {E} `{tl2E V -< E} (n : nat) (k : K) (v : V k) (wv : nat) (l : bool): itree E unit :=
-  trigger (WriteTVarTL2 (mk_tvar V n k) v wv l).
-
-
-
-Definition is_none {A} (o : option A) : bool := match o with None => true | Some _ => false end.
-
-Definition to_list {M A} `{Foldable M A} : M -> list A := fold cons [].
-
-(* Implements transactions with the Transactional Locking II algorithm *)
-Definition tl2 {K} {V : K -> Type} {M}
-  `{HMap (pkey K nat) (pkey_type V) M} `{Foldable M (sigT (@pkey_type K nat V))} {E} `{tl2E V -< E} `{errorE -< E}:
-  transactionE (stmE V) ~> itree E :=
-  fun A e =>
-    match e with
-    | Transaction t0 =>
-        (* sample global version-clock *)
-        rv <- trigger GetVersionClock ;;
-        (* run through a speculative execution *)
-        let m : stateT (_ * M) (failT (itree E)) _ :=
-          interp (handle_tvar_log_tl2 rv) t0 in
-        res <- m ([], HMap.empty) ;;
-        match res with
-        | None => Ret None (* transaction retried or read a failure state *)
-        | Some ((s_r, m_w), a) =>
-            (* lock the write-set *)
-            (* sorts the locks so that we avoid deadlocks *)
-            let locks := Mergesort.sort (fun x y => Nat.leb (snd (projT1 x)) (snd (projT1 y))) (to_list m_w) in
-            fold (fun '(existT _ (k, n) _) (acc : itree E unit) =>
-                    spinlock_tvar (mk_tvar V n k) ;; acc)
-                 (Ret tt)
-                 locks ;;
-                (* increment the global version-clock *)
-                wv <- trigger IncVersionClock ;;
-                (* validate the read-set *)
-                validated <- fold (fun '(k, n) t =>
-                                    '(_, ver, l) <- trigger (ReadTVarTL2 (mk_tvar V n k)) ;;
-                                    (* check that if the lock is held, it is because we locked it and that it hasn't been written to *)
-                                    if (l && is_none (lookup (k, n) m_w)) || (rv <? ver)
-                                    then Ret false
-                                    else t)
-                                  (Ret true) s_r ;;
-                if negb validated
-                then
-                  (* release the write locks *)
-                  fold (fun '(existT _ (k, n) _) acc => trigger (UnlockTVar (mk_tvar V n k)) ;; acc)
-                       (Ret tt) m_w ;;
-                  Ret None
-                else
-                  (* commit and release the locks *)
-                  fold (fun '(existT _ p v) t =>
-                                (* write also sets the lock bit to unlocked *)
-                                trigger (WriteTVarTL2 (mk_tvar V (snd p) (fst p)) v wv false) ;;
-                                t)
-                      (Ret tt) m_w ;;
-                  Ret (Some a)
-        end
-    end.
-
-
-
-Definition h_tl2 {E} `{errorE -< E} {K} {V : K -> Type} M
-  `{HMap (pkey K nat) (fun p => (V (fst p) * nat * bool)%type) M}
-  `{Foldable M (sigT (fun p : K * nat => (V (fst p) * nat * bool)%type))}:
-  tl2E V ~> stateT (nat * M) (itree E) :=
-  fun _ e '(vc, m) =>
-    match e with
-    | GetVersionClock => Ret (vc, m, vc)
-    | IncVersionClock => Ret (S vc, m, S vc)
-    | NewTVarTL2 k v =>
-        let n := S (fold (fun '(existT _ (_, n) _) acc => max n acc) 0 m) in
-        Ret (vc, add (k, n) (v, vc, false) m, mk_tvar V n k)
-    | ReadTVarTL2 x =>
-        let '(mk_tvar _ n k) := x in
-        match lookup (k, n) m with
-        | Some v => Ret (vc, m, v)
-        | None => error "ReadTVarTL2 lookup failed" (* error *)
-        end
-    | WriteTVarTL2 x v wv l =>
-        (let '(mk_tvar _ n k) := x in
-         fun (v : V k) => Ret (vc, add (k, n) (v, wv, l) m, tt)) v
-    | TryLockTVar x =>
-        let '(mk_tvar _ n k) := x in
-        match lookup (k, n) m with
-        | Some (v, wv, l) =>
-            if (l : bool)
-            then Ret (vc, m, false)
-            else Ret (vc, add (k, n) (v, wv, true) m, true)
-        | None => error "h_tl2 TryLockTVar lookup failed" (* error *)
-        end
-    | UnlockTVar (mk_tvar _ n k) =>
-        match lookup (k, n) m with
-        | Some (v, wv, l) =>
-          Ret (vc, add (k, n) (v, wv, false) m, tt)
-        | None => error "h_tl2 UnlockTVar lookup failed"
-        end
-    end.
-
-Definition handle_tvars {E} {K} (V : K -> Type) M
-  `{HMap (pkey K nat) (pkey_type V) M} `{Foldable M (sigT (@pkey_type K nat V))}:
-  tvarE V ~> stateT M (itree E) :=
-  fun _ t m =>
-    match t with
-    | NewTVar k v =>
-        let n := S (fold (fun '(existT _ (_, n) _) acc => max n acc) 0 m) in
-        Ret (add (k, n) v m, mk_tvar V n k)
-    | ReadTVar x =>
-        let '(mk_tvar _ n k) := x in
-        match lookup (k, n) m with
-        | Some v => Ret (m, v)
-        | None => ITree.spin (* error *)
-        end
-    | WriteTVar x v =>
-        (let '(mk_tvar _ n k) := x in
-         fun (v : V k) => Ret (add (k, n) v m, tt)) v
-    end.
-
-Definition h_tvars_tl2 {K} (V : K -> Type):
-  tvarE V ~> itree (tl2E V) :=
-  fun _ e =>
-    match e with
-    | NewTVar k v => ITree.trigger (NewTVarTL2 k v)
-    | ReadTVar x =>
-        '(v, _, _) <- trigger (ReadTVarTL2 x) ;;
-        Ret v
-    | WriteTVar x v => ITree.spin (* error *)
-    end.
-
-
-
-(* Scheduler implementations should be such that 0 getting chosen infinitely often will ensure that every thread gets scheduled *)
-Variant scheduleE : Type -> Type :=
-| Schedule (n : nat) : scheduleE {m : nat | m < n}.
-
-Definition h_rr {E} : scheduleE ~> itree E :=
-  fun _ e =>
-    match e with
-    | Schedule n =>
-        match n with
-        | 0 => ITree.spin (* error *)
-        | S m => Ret (exist _ 0 (PeanoNat.Nat.lt_0_succ m))
-        end
-    end.
-
-Fixpoint signth {A} (l : list A) (n : {m : nat | m < length l}) : A :=
-  match l, n with
-  | [], exist _ m H => False_rect _ (PeanoNat.Nat.nlt_0_r m H)
-  | (v :: l), exist _ m H =>
-    match m with
-    | 0 => fun _ => v
-    | S m => fun H : S m < S (length l) => signth l (exist _ m (PeanoNat.lt_S_n _ _ H))
-    end H
-  end.
-
-
-
-Inductive parE E : Type -> Type :=
-| Par : forall {A B} (t1 : itree (parE E +' E) A) (t2 : itree (parE E +' E) B), parE E (A * B).
-
-Definition par {E F} `{parE F -< E} {A B} (t1 : itree (parE F +' F) A) (t2 : itree (parE F +' F) B) : itree E (A * B) :=
-  trigger (Par _ t1 t2).
-
-Inductive par_tree E R :=
-| Split {A B} (b : bool) (t1 : par_tree E A) (t2 : par_tree E B) (k : A * B -> itree (parE E +' E) R) : par_tree E R
-| LeftDone {A B} (a : A) (t2 : par_tree E B) (k : A * B -> itree (parE E +' E) R) : par_tree E R
-| RightDone {A B} (t1 : par_tree E A) (b : B) (k : A * B -> itree (parE E +' E) R) : par_tree E R
-| Leaf (t : itree (parE E +' E) R) : par_tree E R.
-
-Inductive par_tree_ctx E R : Type -> Type :=
-| MT : par_tree_ctx E R R
-| SplitR {A B T} (b : bool) (t1 : par_tree E A) (k : A * B -> itree (parE E +' E) T) (pk : par_tree_ctx E R T) : par_tree_ctx E R B
-| SplitL {A B T} (b : bool) (t2 : par_tree E B) (k : A * B -> itree (parE E +' E) T) (pk : par_tree_ctx E R T) : par_tree_ctx E R A
-| LeftDoneCtx {A B T} (a : A) (k : A * B -> itree (parE E +' E) T) (pk : par_tree_ctx E R T) : par_tree_ctx E R B
-| RightDoneCtx {A B T} (b : B) (k : A * B -> itree (parE E +' E) T) (pk : par_tree_ctx E R T) : par_tree_ctx E R A.
-
-Fixpoint plug_par_tree_ctx {E R T} (pk : par_tree_ctx E R T) (pt : par_tree E T) : par_tree E R :=
-  match pk, pt with
-  | MT _ _, pt => pt
-  | SplitR _ _ b t1 k pk, pt => plug_par_tree_ctx pk (Split _ _ b t1 pt k)
-  | SplitL _ _ b t2 k pk, pt => plug_par_tree_ctx pk (Split _ _ b pt t2 k)
-  | LeftDoneCtx _ _ a k pk, pt => plug_par_tree_ctx pk (LeftDone _ _ a pt k)
-  | RightDoneCtx _ _ b k pk, pt => plug_par_tree_ctx pk (RightDone _ _ pt b k)
-  end.
-
-(* needs to randomly select a leaf from the par tree, then observe it and put it back *)
-CoFixpoint schedule_par {E R} (pt : par_tree E R) : itree (scheduleE +' E) R :=
-  let fix find_leaf {T} (pt : par_tree E T) (pk : par_tree_ctx E R T)
-    : itree (scheduleE +' E) (sigT (fun T => (par_tree_ctx E R T * itree (parE E +' E) T)%type)) :=
-    match pt with
-    | Split _ _ b t1 t2 k =>
-        Vis (inl1 (Schedule 2))
-            (fun (n : {m : nat | m < 2}) =>
-              let '(exist _ n _) := n in
-              (* use the boolean to ensure that both branches get scheduled for rr scheduler *)
-              if xorb (n =? 0) b
-              then find_leaf t1 (SplitL _ _ true t2 k pk)
-              else find_leaf t2 (SplitR _ _ false t1 k pk))
-    | LeftDone _ _ a t2 k => find_leaf t2 (LeftDoneCtx _ _ a k pk)
-    | RightDone _ _ t1 b k => find_leaf t1 (RightDoneCtx _ _ b k pk)
-    | Leaf _ _ t => Ret (existT _ _ (pk, t))
-    end in
-  '(existT _ _ (pk, t)) <- find_leaf pt (MT _ _) ;;
-  match observe t with
-  | RetF v =>
-      match pk, v with
-      | MT _ _, a => Ret a
-      | SplitR _ _ _ t1 k pk, b => Tau (schedule_par (plug_par_tree_ctx pk (RightDone _ _ t1 b k)))
-      | SplitL _ _ _ t2 k pk, a => Tau (schedule_par (plug_par_tree_ctx pk (LeftDone _ _ a t2 k)))
-      | LeftDoneCtx _ _ a k pk, b => Tau (schedule_par (plug_par_tree_ctx pk (Leaf _ _ (k (a, b)))))
-      | RightDoneCtx _ _ b k pk, a => Tau (schedule_par (plug_par_tree_ctx pk (Leaf _ _ (k (a, b)))))
-      end
-  | TauF t => Tau (schedule_par (plug_par_tree_ctx pk (Leaf _ _ t)))
-  | VisF (inl1 e) k =>
-      match e, k with
-      | Par _ t1 t2, k => Tau (schedule_par (plug_par_tree_ctx pk (Split _ _ false (Leaf _ _ t1) (Leaf _ _ t2) k)))
-      end
-  | VisF (inr1 e) k => Vis (inr1 e) (fun x => schedule_par (plug_par_tree_ctx pk (Leaf _ _ (k x))))
-  end.
-
-
-
-Variant forkE : Type -> Type :=
-| Fork : forkE bool.
-
-Definition fork {E} `{forkE -< E} (t1 t2 : itree E unit) : itree E unit :=
-  b <- trigger Fork ;;
-  if (b : bool) then t1 else t2.
-
-(* arranged so that a scheduleE handler that always returns 0 will be a round-robin scheduler *)
-CoFixpoint schedule {E F} `{F -< E} (l : list (itree (atomicE F +' forkE +' E) unit)) : itree (scheduleE +' E) unit :=
-  match l with
-  | [] => Ret tt
-  | _ =>
-    Vis (subevent _ (Schedule (length l)))
-        (fun n =>
-          let l1 := firstn (proj1_sig n) l in
-          let l2 := skipn (S (proj1_sig n)) l in
-          let t := signth l n in
-          match observe t with
-          | RetF _ => schedule (l1 ++ l2)
-          | TauF t => schedule (l1 ++ l2 ++ [t])
-          | VisF (inl1 e) k =>
-              match e, k with
-              | Atomic t, k => a <- translate subevent t ;; schedule (l1 ++ l2 ++ [k a])
-              end
-          | VisF (inr1 (inl1 e)) k =>
-              match e, k with
-              | Fork, k => schedule (l1 ++ l2 ++ [k true; k false])
-              end
-          | VisF (inr1 (inr1 e)) k => Vis (subevent _ e) (fun x => schedule (l1 ++ l2 ++ [k x]))
-          end)
-  end.
-
-Definition schedule_rr {E F} `{F -< E} (l : list (itree (atomicE F +' forkE +' E) unit)) : itree E unit :=
-  interp (case_ h_rr (id_ _)) (schedule l).
-
-Definition schedule_par_rr {E R} (pt : par_tree E R) : itree E R :=
-  interp (case_ h_rr (id_ _)) (schedule_par pt).
-
-Definition newTVar {E K V} `{tvarE V -< E} (k : K) (a : V k) : itree E (TVar V (V k)) := embed (NewTVar k a).
-Definition readTVar {E K} {V : K -> Type} `{tvarE V -< E} {A} (v : TVar V A) : itree E A := embed (ReadTVar v).
-Definition writeTVar {E K} {V : K -> Type} `{tvarE V -< E} {A} (v : TVar V A) (a : A) : itree E unit := embed (WriteTVar v a).
+Definition newTVar {K V} (k : K) (a : V k) : itree (stmE V) (TVar V (V k)) := trigger (inr1 (NewTVar k a)).
+Definition readTVar {K} {V : K -> Type} {A} (v : TVar V A) : itree (stmE V) A := trigger (inr1 (ReadTVar v)).
+Definition writeTVar {K} {V : K -> Type} {A} (v : TVar V A) (a : A) : itree (stmE V) unit := trigger (inr1 (WriteTVar v a)).
 
 Definition check {K} {V : K -> Type} (b : bool) : itree (stmE V) unit :=
   if b then Ret tt else retry.
@@ -540,179 +96,7 @@ Definition modifyTVar {K} {V : K -> Type} {A : Type} (a : TVar V A) (f : A -> A)
   writeTVar a (f val) ;;
   Ret tt.
 
-
-
-Section example.
-
-  #[global] Instance EqDec_unit : EqDec unit eq :=
-    fun x y => match x, y with tt, tt => left eq_refl end.
-
-  Definition nats (_ : unit) : Type := nat.
-
-  Definition fib_trans (x0 x1 : TVar nats nat): itree (stmE nats) unit :=
-    v0 <- readTVar x0 ;;
-    v1 <- readTVar x1 ;;
-    writeTVar x0 v1 ;;
-    writeTVar x1 (v0 + v1).
-
-  Definition fib (n : nat) : itree (runStmE nats +' forkE) unit :=
-    '(x, y) <- atomically (
-      x <- newTVar tt 0 ;;
-      y <- newTVar tt 1 ;;
-      Ret (x, y)) ;;
-    (fix fib_ n :=
-      match n with
-      | 0 => Ret tt
-      | S n => fork (atomically (fib_trans x y)) (fib_ n)
-      end) n.
-
-
-
-  Definition run_atomically {K} {V : K -> Type} {E A} (t0 : itree (runStmE V +' E) A):
-    itree (transactionE (stmE V) +' E) A :=
-    interp (bimap h_atomically (id_ _)) t0.
-
-  Definition run_atomic_transactions {K} `{EqDec K eq} {V : K -> Type}
-    (t1 : itree (transactionE (stmE V) +' forkE) unit):
-    itree void1 (halist (pkey K nat) (pkey_type V) * unit) :=
-    let t2 : itree (atomicE (tvarE V) +' forkE +' tvarE V) unit := translate (bimap atomic_transactions subevent) t1 in
-    let t3 : stateT _ _ _ := interp (handle_tvars _ _) (schedule_rr [t2]) in
-    t3 HMap.empty.
-
-
-
-  Definition h_trigger {E F} `{E -< F}: Handler E F :=
-    fun _ e => trigger e.
-
-  Definition run_single_lock {K} `{EqDec K eq} {V : K -> Type}
-    (t1 : itree (transactionE (stmE V) +' forkE) unit):
-    itree void1 (halist (pkey K nat) (pkey_type V) * (bool * unit)) :=
-    let t2 : itree (atomicE void1 +' forkE +' lockE +' tvarE V) unit :=
-      interp (case_ single_global_lock h_trigger) t1 in
-    let t3 := schedule_rr [t2] in
-    let t4 : stateT bool (itree (tvarE V)) unit := interp (case_ h_lock pure_state) t3 in
-    let t5 : stateT _ (itree void1) _ := interp (handle_tvars _ _) (t4 false) in
-    t5 HMap.empty.
-
-
-
-  Definition run_tl2 {K} `{EqDec K eq} {V : K -> Type}
-    (t1 : itree (transactionE (stmE V) +' forkE) unit)
-    : itree errorE (nat * halist (pkey K nat) (fun p => (V (fst p) * nat * bool)%type) * unit) :=
-    let t2 : itree (atomicE void1 +' forkE +' tl2E V +' errorE) unit :=
-      interp (case_ tl2 h_trigger) t1 in
-    let t3 : itree (tl2E V +' errorE) unit := schedule_rr [t2] in
-    let t4 : stateT _ (itree errorE) _ :=
-      interp (case_ (h_tl2 _) pure_state) t3 in
-    t4 (0, HMap.empty).
-
-
-
-  Variant result (E : Type -> Type) (A : Type) :=
-  | Val : A -> result E A
-  | NotYet : result E A
-  | Event : forall {X}, E X -> result E A.
-
-  Arguments Val {E A} (a).
-  Arguments NotYet {E A}.
-  Arguments Event {E A} {X} (e).
-
-  Definition force {E A} (n : nat) (t : itree E A) : result E A :=
-    match observe (burn n t) with
-    | RetF a => Val a
-    | TauF _ => NotYet
-    | VisF e _ => Event e
-    end.
-
-  Definition unwrap {E A} : option A -> itree E A :=
-    fun o => match o with None => ITree.spin | Some a => Ret a end.
-
-  Compute (force 178 (run_atomic_transactions (run_atomically (fib 8)))).
-  Compute (force 1000 (run_single_lock (run_atomically (fib 8)))).
-  Compute (force 1874 (run_tl2 (run_atomically (fib 8)))).
-
-  Definition read_test : itree (runStmE nats +' forkE) unit :=
-    x <- atomically (newTVar tt 21) ;;
-    atomically (readTVar x) ;;
-    Ret tt.
-
-  Definition write_test : itree (runStmE nats +' forkE) unit :=
-    x <- atomically (newTVar tt 22) ;;
-    atomically (writeTVar x 23).
-
-  Definition inc_test : itree (runStmE nats +' forkE) unit :=
-    x <- atomically (newTVar tt 0) ;;
-    atomically (v <- readTVar x ;; writeTVar x (S v)).
-
-  Compute (force 1000 (run_tl2 (run_atomically read_test))).
-  Compute (force 1000 (run_tl2 (run_atomically write_test))).
-  Compute (force 1000 (run_tl2 (run_atomically inc_test))).
-
-  Definition takeMVar {K} {V : K -> Type} {A} (t : TVar V (option A)) : itree (stmE V) A :=
-    v <- readTVar t ;;
-    match v with
-    | None => retry
-    | Some a => writeTVar t None ;; Ret a
-    end.
-
-  Definition putMVar {K} {V : K -> Type} {A} (t : TVar V (option A)) (a : A) : itree (stmE V) unit :=
-    v <- readTVar t ;;
-    match v with
-    | None => writeTVar t (Some a)
-    | Some _ => retry
-    end.
-
-  Inductive Types :=
-  | Nat : Types
-  | Opt : Types -> Types.
-
-  Definition decide_types (x y : Types) : {x = y} + {x <> y}.
-    decide equality.
-  Defined.
-
-  #[global] Instance EqDec_Types : EqDec Types eq := decide_types.
-
-  Fixpoint Types_Type (type : Types) : Type :=
-    match type with
-    | Nat => nat
-    | Opt t => option (Types_Type t)
-    end.
-
-  Definition message_passing : itree (runStmE Types_Type +' forkE) unit :=
-    mv <- atomically (newTVar (Opt Nat) None) ;;
-    done <- atomically (newTVar Nat 0) ;;
-    fork (v1 <- atomically (takeMVar mv) ;; v2 <- atomically (takeMVar mv) ;; atomically (putMVar mv (v1 + v2)))
-         (atomically (putMVar mv 3) ;; atomically (putMVar mv 4) ;; atomically (r <- takeMVar mv ;; writeTVar done r)).
-
-  Definition message_passing_simple : itree (runStmE Types_Type +' forkE) unit :=
-    mv <- atomically (newTVar (Opt Nat) None) ;;
-    done <- atomically (newTVar Nat 0) ;;
-    fork (v1 <- atomically (takeMVar mv) ;; atomically (putMVar mv (v1 * v1)))
-         (atomically (putMVar mv 3) ;; atomically (r <- takeMVar mv ;; writeTVar done r)).
-
-  Definition message_passing_simpler : itree (runStmE Types_Type +' forkE) unit :=
-    mv <- atomically (newTVar (Opt Nat) None) ;;
-    done <- atomically (newTVar Nat 0) ;;
-    fork (v1 <- atomically (takeMVar mv) ;; atomically (writeTVar done (v1 * v1)))
-         (atomically (putMVar mv 3)).
-
-  Compute (force 100 (run_atomic_transactions (run_atomically message_passing_simpler))).
-  Compute (force 100 (run_atomic_transactions (run_atomically message_passing_simple))).
-  Compute (force 100 (run_atomic_transactions (run_atomically message_passing))).
-  Compute (force 200 (run_single_lock (run_atomically message_passing_simpler))).
-  Compute (force 200 (run_single_lock (run_atomically message_passing_simple))).
-  Compute (force 300 (run_single_lock (run_atomically message_passing))).
-  Compute (force 1000 (run_tl2 (run_atomically message_passing_simpler))).
-  Compute (force 1000 (run_tl2 (run_atomically message_passing_simple))).
-  Compute (force 1000 (run_tl2 (run_atomically message_passing))).
-
-  (* TODO: tests with orElse *)
-
-End example.
-
-
-
 Crane Extract Inlined Constant atomically => "stm::atomically([&] { return %a0; })".
-Crane Extract Inlined Constant orElse => "stm::orElse<%t0>(%a0, %a1)".
-Crane Extract Inlined Constant retry => "stm::retry<%t0>()".
+(*Crane Extract Inlined Constant orElse => "stm::orElse<%t0>(%a0, %a1)".*)
+Crane Extract Inlined Constant retry => "stm::retry<%t2>()".
 Crane Extract Inlined Constant newTVar => "stm::newTVar(%a1)".
