theories/Monads/STM/ForkDefs.v
@@ -1,0 +1,51 @@
+From Crane Require Import Monads.ITree Monads.STM.Schedule.
+
+From Stdlib Require Import List.
+
+Import ListNotations.
+
+From ExtLib Require Import Structures.Monad.
+
+From ITree Require Import Basics.CategoryOps.
+
+Open Scope itree_scope.
+
+Variant atomicE E : Type -> Type :=
+| Atomic : forall {A} (t : itree E A), atomicE E A.
+
+Arguments Atomic {E} {A} (_).
+
+Variant forkE : Type -> Type :=
+| Fork : forkE bool.
+
+Definition fork {E} `{forkE -< E} (t1 t2 : itree E unit) : itree E unit :=
+  b <- trigger Fork ;;
+  if (b : bool) then t1 else t2.
+
+(* arranged so that a scheduleE handler that always returns 0 will be a round-robin scheduler *)
+CoFixpoint schedule {E F} `{F -< E} (l : list (itree (atomicE F +' forkE +' E) unit)) : itree (scheduleE +' E) unit :=
+  match l with
+  | [] => Ret tt
+  | _ =>
+    Vis (subevent _ (Schedule (length l)))
+        (fun n =>
+          let l1 := firstn (proj1_sig n) l in
+          let l2 := skipn (S (proj1_sig n)) l in
+          let t := signth l n in
+          match observe t with
+          | RetF _ => schedule (l1 ++ l2)
+          | TauF t => schedule (l1 ++ l2 ++ [t])
+          | VisF (inl1 e) k =>
+              match e, k with
+              | Atomic t, k => a <- translate subevent t ;; schedule (l1 ++ l2 ++ [k a])
+              end
+          | VisF (inr1 (inl1 e)) k =>
+              match e, k with
+              | Fork, k => schedule (l1 ++ l2 ++ [k true; k false])
+              end
+          | VisF (inr1 (inr1 e)) k => Vis (subevent _ e) (fun x => schedule (l1 ++ l2 ++ [k x]))
+          end)
+  end.
+
+Definition schedule_rr {E F} `{F -< E} (l : list (itree (atomicE F +' forkE +' E) unit)) : itree E unit :=
+  interp (case_ h_rr (id_ _)) (schedule l).
