theories/Monads/STM/ParDefs.v
@@ -1,0 +1,74 @@
+From Crane Require Import Monads.ITree Monads.STM.Schedule.
+
+From Stdlib Require Import Arith.PeanoNat Bool.Bool Classes.EquivDec.
+
+From ITree Require Import Basics.CategoryOps.
+
+
+Inductive parE E : Type -> Type :=
+| Par : forall {A B} (t1 : itree (parE E +' E) A) (t2 : itree (parE E +' E) B), parE E (A * B).
+
+Definition par {E F} `{parE F -< E} {A B} (t1 : itree (parE F +' F) A) (t2 : itree (parE F +' F) B) : itree E (A * B) :=
+  trigger (Par _ t1 t2).
+
+Inductive par_tree E R :=
+| Split {A B} (b : bool) (t1 : par_tree E A) (t2 : par_tree E B) (k : A * B -> itree (parE E +' E) R) : par_tree E R
+| LeftDone {A B} (a : A) (t2 : par_tree E B) (k : A * B -> itree (parE E +' E) R) : par_tree E R
+| RightDone {A B} (t1 : par_tree E A) (b : B) (k : A * B -> itree (parE E +' E) R) : par_tree E R
+| Leaf (t : itree (parE E +' E) R) : par_tree E R.
+
+Inductive par_tree_ctx E R : Type -> Type :=
+| MT : par_tree_ctx E R R
+| SplitR {A B T} (b : bool) (t1 : par_tree E A) (k : A * B -> itree (parE E +' E) T) (pk : par_tree_ctx E R T) : par_tree_ctx E R B
+| SplitL {A B T} (b : bool) (t2 : par_tree E B) (k : A * B -> itree (parE E +' E) T) (pk : par_tree_ctx E R T) : par_tree_ctx E R A
+| LeftDoneCtx {A B T} (a : A) (k : A * B -> itree (parE E +' E) T) (pk : par_tree_ctx E R T) : par_tree_ctx E R B
+| RightDoneCtx {A B T} (b : B) (k : A * B -> itree (parE E +' E) T) (pk : par_tree_ctx E R T) : par_tree_ctx E R A.
+
+Fixpoint plug_par_tree_ctx {E R T} (pk : par_tree_ctx E R T) (pt : par_tree E T) : par_tree E R :=
+  match pk, pt with
+  | MT _ _, pt => pt
+  | SplitR _ _ b t1 k pk, pt => plug_par_tree_ctx pk (Split _ _ b t1 pt k)
+  | SplitL _ _ b t2 k pk, pt => plug_par_tree_ctx pk (Split _ _ b pt t2 k)
+  | LeftDoneCtx _ _ a k pk, pt => plug_par_tree_ctx pk (LeftDone _ _ a pt k)
+  | RightDoneCtx _ _ b k pk, pt => plug_par_tree_ctx pk (RightDone _ _ pt b k)
+  end.
+
+(* needs to randomly select a leaf from the par tree, then observe it and put it back *)
+CoFixpoint schedule_par {E R} (pt : par_tree E R) : itree (scheduleE +' E) R :=
+  let fix find_leaf {T} (pt : par_tree E T) (pk : par_tree_ctx E R T)
+    : itree (scheduleE +' E) (sigT (fun T => (par_tree_ctx E R T * itree (parE E +' E) T)%type)) :=
+    match pt with
+    | Split _ _ b t1 t2 k =>
+        Vis (inl1 (Schedule 2))
+            (fun (n : {m : nat | m < 2}) =>
+              let '(exist _ n _) := n in
+              (* use the boolean to ensure that both branches get scheduled for rr scheduler *)
+              if xorb (n =? 0) b
+              then find_leaf t1 (SplitL _ _ true t2 k pk)
+              else find_leaf t2 (SplitR _ _ false t1 k pk))
+    | LeftDone _ _ a t2 k => find_leaf t2 (LeftDoneCtx _ _ a k pk)
+    | RightDone _ _ t1 b k => find_leaf t1 (RightDoneCtx _ _ b k pk)
+    | Leaf _ _ t => Ret (existT _ _ (pk, t))
+    end in
+  '(existT _ _ (pk, t)) <- find_leaf pt (MT _ _) ;;
+  match observe t with
+  | RetF v =>
+      match pk, v with
+      | MT _ _, a => Ret a
+      | SplitR _ _ _ t1 k pk, b => Tau (schedule_par (plug_par_tree_ctx pk (RightDone _ _ t1 b k)))
+      | SplitL _ _ _ t2 k pk, a => Tau (schedule_par (plug_par_tree_ctx pk (LeftDone _ _ a t2 k)))
+      | LeftDoneCtx _ _ a k pk, b => Tau (schedule_par (plug_par_tree_ctx pk (Leaf _ _ (k (a, b)))))
+      | RightDoneCtx _ _ b k pk, a => Tau (schedule_par (plug_par_tree_ctx pk (Leaf _ _ (k (a, b)))))
+      end
+  | TauF t => Tau (schedule_par (plug_par_tree_ctx pk (Leaf _ _ t)))
+  | VisF (inl1 e) k =>
+      match e, k with
+      | Par _ t1 t2, k => Tau (schedule_par (plug_par_tree_ctx pk (Split _ _ false (Leaf _ _ t1) (Leaf _ _ t2) k)))
+      end
+  | VisF (inr1 e) k => Vis (inr1 e) (fun x => schedule_par (plug_par_tree_ctx pk (Leaf _ _ (k x))))
+  end.
+
+
+
+Definition schedule_par_rr {E R} (pt : par_tree E R) : itree E R :=
+  interp (case_ h_rr (id_ _)) (schedule_par pt).
