theories/Monads/STM/STMModels.v
@@ -1,0 +1,479 @@
+From Corelib Require Import PrimString.
+From Crane Require Import Monads.ITree Monads.STMDefs Monads.STM.ForkDefs.
+
+From Stdlib Require Import Arith.PeanoNat Bool.Bool Classes.EquivDec List.
+
+Import ListNotations.
+
+From ExtLib Require Import Data.List Structures.Reducible.
+
+From ITree Require Import Basics.Basics Basics.CategoryOps Events.State Events.FailFacts.
+
+Import Basics.Monads.
+
+From Crane.Utils Require Import HMap HAList Mergesort.
+
+Definition pkey (K J : Type) := (K * J)%type.
+Definition pkey_type {K J} (V : K -> Type) (pk : pkey K J) := V (fst pk).
+
+Definition commit_log {K} (V : K -> Type) {M} `{Foldable M (sigT (pkey_type V))} {E} `{H : tvarE V -< E} : M -> itree E unit :=
+  fold (fun '(existT _ (k, n) v) acc => Vis (subevent (H := H) _ (WriteTVar (mk_tvar V n k) v)) (fun _ => acc)) (Ret tt).
+
+Definition handle_tvar_log {K} {V : K -> Type} {M} `{HMap (pkey K nat) (pkey_type V) M} {E} `{H : tvarE V -< E}
+  (m : M) : forall {A}, tvarE V A -> itree E (A * M) :=
+  fun _ t =>
+    match t with
+    | NewTVar k v => Vis (subevent (H := H) _ (NewTVar k v)) (fun tv => Ret (tv, m))
+    | ReadTVar tv =>
+        (let '(mk_tvar _ n k) in TVar _ T := tv return TVar V T -> itree E (T * M) in
+          match lookup (k, n) m with
+          | Some v => fun _ => Ret (v, m)
+          | None => fun tv => Vis (subevent (H := H) _ (ReadTVar tv)) (fun v => Ret (v, m))
+          end) tv
+    | WriteTVar (mk_tvar _ n k) v => Ret (tt, add (k, n) v m)
+    end.
+
+
+
+Variant transactionE E : Type -> Type :=
+| Transaction : forall {A}, itree E A -> transactionE E (option A).
+
+Arguments Transaction {E} {A} (_).
+
+
+
+Definition h_atomically {K} {V : K -> Type} {E} `{transactionE (stmE V) -< E} : runStmE V ~> itree E :=
+  fun _ e =>
+    match e with
+    | Atomically t =>
+        ITree.iter (fun _ =>
+                      oa <- trigger (Transaction t) ;;
+                      match oa with
+                      | None => Ret (inl tt)
+                      | Some a => Ret (inr a)
+                      end) tt
+    end.
+
+
+
+Definition h_stm_write_log {K} {V : K -> Type} {M} `{HMap (pkey K nat) (pkey_type V) M} {E} `{tvarE V -< E}:
+  stmE V ~> stateT M (failT (itree E)) :=
+  fun _ e m =>
+    match e with
+    | inl1 Retry => Ret None
+    | inr1 e =>
+        '(a, m) <- handle_tvar_log m e ;;
+        Ret (Some (m, a))
+    end.
+
+(* TODO: generalize to any HMap *)
+(* Implements transactions by executing them atomically (blocks all other threads from executing until it is finished) *)
+Definition atomic_transactions {K} {V : K -> Type} `{EqDec K eq}: transactionE (stmE V) ~> atomicE (tvarE V) :=
+  fun _ e =>
+    match e with
+    | Transaction t =>
+        let m : stateT (halist (pkey K nat) (pkey_type V)) (failT (itree (tvarE V))) _ :=
+          interp h_stm_write_log t in
+        Atomic (res <- m [] ;;
+                match res with
+                | Some (m, a) =>
+                    commit_log _ m ;;
+                    Ret (Some a)
+                | None => Ret None
+                end)
+    end.
+
+Variant lockE : Type -> Type :=
+| TryLock : lockE bool
+| Unlock : lockE unit.
+
+Definition spinlock {E} `{lockE -< E} : itree E unit :=
+  ITree.iter (fun n => b <- trigger TryLock ;; if (b : bool) then Ret (inr tt) else Ret (inl (S n))) 0.
+
+(* TODO: generalize to any HMap *)
+(* implements transactions through a single global lock that is acquired before transaction execution *)
+Definition single_global_lock {K} {V : K -> Type} `{EqDec K eq} {E} `{lockE -< E} `{tvarE V -< E}:
+  transactionE (stmE V) ~> itree E :=
+  fun _ e =>
+    match e with
+    | Transaction t =>
+        spinlock ;;
+        let m : stateT (halist (pkey K nat) (pkey_type V)) (failT (itree E)) _ :=
+          interp h_stm_write_log t in
+        res <- m [] ;;
+        match res with
+        | Some (m, a) =>
+            commit_log _ m ;;
+            trigger Unlock ;;
+            Ret (Some a)
+        | None =>
+            trigger Unlock ;;
+            Ret None
+        end
+    end.
+
+Definition h_lock {E} : lockE ~> stateT bool (itree E) :=
+  fun _ e l =>
+    match e with
+    | TryLock => Ret (true, negb l)
+    | Unlock => Ret (false, tt)
+    end.
+
+
+
+
+Variant tl2E {K} (V : K -> Type) : Type -> Type :=
+| GetVersionClock : tl2E V nat
+| IncVersionClock : tl2E V nat
+| NewTVarTL2 : forall (k : K), V k -> tl2E V (TVar V (V k))
+| ReadTVarTL2 : forall {A}, TVar V A -> tl2E V (A * nat * bool)
+| WriteTVarTL2 : forall {A}, TVar V A -> A -> nat -> bool -> tl2E V unit
+| TryLockTVar : forall {A}, TVar V A -> tl2E V bool
+| UnlockTVar : forall {A}, TVar V A -> tl2E V unit.
+
+Arguments GetVersionClock {K} {V}.
+Arguments IncVersionClock {K} {V}.
+Arguments NewTVarTL2 {K} {V} (_ _).
+Arguments ReadTVarTL2 {K} {V} {A} (_).
+Arguments WriteTVarTL2 {K} {V} {A} (_ _ _ _).
+Arguments TryLockTVar {K} {V} {A} (_).
+Arguments UnlockTVar {K} {V} {A} (_).
+
+
+
+(* a blocking spinlock *)
+Definition spinlock_tvar {K} {V : K -> Type} {E} `{tl2E V -< E} {A} (x : TVar V A) : itree E unit :=
+  ITree.iter (fun _ => b <- trigger (TryLockTVar x) ;; if (b : bool) then Ret (inr tt) else Ret (inl tt)) tt.
+
+
+
+Variant errorE : Type -> Type :=
+| Error (msg : string) : errorE void.
+
+Definition error {E A} `{errorE -< E} (msg : string) : itree E A :=
+  Vis (subevent _ (Error msg)) (fun (x : void) => match x with end).
+
+
+
+Definition handle_tvar_log_tl2 {K} {V : K -> Type} {M} `{HMap (pkey K nat) (pkey_type V) M} {E} `{H : tl2E V -< E}
+  (rv : nat) : stmE V ~> stateT (list (pkey K nat) * M) (failT (itree E)) :=
+  fun _ t '(s_r, m_w) =>
+    match t with
+    | inl1 Retry => Ret None
+    | inr1 e =>
+      match e with
+      | NewTVar k v => Vis (subevent (H := H) _ (NewTVarTL2 k v)) (fun tv => Ret (Some ((s_r, m_w), tv)))
+      | ReadTVar tv =>
+          (let '(mk_tvar _ n k) in TVar _ T := tv return TVar V T -> itree E (option ((list (pkey K nat) * M) * T)) in
+            match lookup (k, n) m_w with
+            | Some v => fun _ => Ret (Some ((s_r, m_w), v))
+            | None => fun tv =>
+                '(v, ver, l) <- Vis (subevent (H := H) _ (ReadTVarTL2 tv)) (fun x => Ret x);;
+                if l || (rv <? ver)
+                then Ret None
+                else Ret (Some (((k, n) :: s_r, m_w), v))
+            end) tv
+      | WriteTVar (mk_tvar _ n k) v => Ret (Some ((s_r, add (k, n) v m_w), tt))
+      end
+    end.
+
+Definition write_tl2 {K} (V : K -> Type) {E} `{tl2E V -< E} (n : nat) (k : K) (v : V k) (wv : nat) (l : bool): itree E unit :=
+  trigger (WriteTVarTL2 (mk_tvar V n k) v wv l).
+
+
+
+Definition is_none {A} (o : option A) : bool := match o with None => true | Some _ => false end.
+
+Definition to_list {M A} `{Foldable M A} : M -> list A := fold cons [].
+
+(* Implements transactions with the Transactional Locking II algorithm *)
+Definition tl2 {K} {V : K -> Type} {M}
+  `{HMap (pkey K nat) (pkey_type V) M} `{Foldable M (sigT (@pkey_type K nat V))} {E} `{tl2E V -< E} `{errorE -< E}:
+  transactionE (stmE V) ~> itree E :=
+  fun A e =>
+    match e with
+    | Transaction t0 =>
+        (* sample global version-clock *)
+        rv <- trigger GetVersionClock ;;
+        (* run through a speculative execution *)
+        let m : stateT (_ * M) (failT (itree E)) _ :=
+          interp (handle_tvar_log_tl2 rv) t0 in
+        res <- m ([], HMap.empty) ;;
+        match res with
+        | None => Ret None (* transaction retried or read a failure state *)
+        | Some ((s_r, m_w), a) =>
+            (* lock the write-set *)
+            (* sorts the locks so that we avoid deadlocks *)
+            let locks := Mergesort.sort (fun x y => Nat.leb (snd (projT1 x)) (snd (projT1 y))) (to_list m_w) in
+            fold (fun '(existT _ (k, n) _) (acc : itree E unit) =>
+                    spinlock_tvar (mk_tvar V n k) ;; acc)
+                 (Ret tt)
+                 locks ;;
+            (* increment the global version-clock *)
+            wv <- trigger IncVersionClock ;;
+            (* validate the read-set *)
+            validated <- fold (fun '(k, n) t =>
+                                '(_, ver, l) <- trigger (ReadTVarTL2 (mk_tvar V n k)) ;;
+                                (* check that if the lock is held, it is because we locked it and that it hasn't been written to *)
+                                if (l && is_none (lookup (k, n) m_w)) || (rv <? ver)
+                                then Ret false
+                                else t)
+                              (Ret true) s_r ;;
+            if negb validated
+            then
+              (* release the write locks *)
+              fold (fun '(existT _ (k, n) _) acc => trigger (UnlockTVar (mk_tvar V n k)) ;; acc)
+                    (Ret tt) m_w ;;
+              Ret None
+            else
+              (* commit and release the locks *)
+              fold (fun '(existT _ p v) t =>
+                            (* write also sets the lock bit to unlocked *)
+                            trigger (WriteTVarTL2 (mk_tvar V (snd p) (fst p)) v wv false) ;;
+                            t)
+                  (Ret tt) m_w ;;
+              Ret (Some a)
+        end
+    end.
+
+
+
+Definition h_tl2 {E} `{errorE -< E} {K} {V : K -> Type} M
+  `{HMap (pkey K nat) (fun p => (V (fst p) * nat * bool)%type) M}
+  `{Foldable M (sigT (fun p : K * nat => (V (fst p) * nat * bool)%type))}:
+  tl2E V ~> stateT (nat * M) (itree E) :=
+  fun _ e '(vc, m) =>
+    match e with
+    | GetVersionClock => Ret (vc, m, vc)
+    | IncVersionClock => Ret (S vc, m, S vc)
+    | NewTVarTL2 k v =>
+        let n := S (fold (fun '(existT _ (_, n) _) acc => max n acc) 0 m) in
+        Ret (vc, add (k, n) (v, vc, false) m, mk_tvar V n k)
+    | ReadTVarTL2 x =>
+        let '(mk_tvar _ n k) := x in
+        match lookup (k, n) m with
+        | Some v => Ret (vc, m, v)
+        | None => error "ReadTVarTL2 lookup failed" (* error *)
+        end
+    | WriteTVarTL2 x v wv l =>
+        (let '(mk_tvar _ n k) := x in
+         fun (v : V k) => Ret (vc, add (k, n) (v, wv, l) m, tt)) v
+    | TryLockTVar x =>
+        let '(mk_tvar _ n k) := x in
+        match lookup (k, n) m with
+        | Some (v, wv, l) =>
+            if (l : bool)
+            then Ret (vc, m, false)
+            else Ret (vc, add (k, n) (v, wv, true) m, true)
+        | None => error "h_tl2 TryLockTVar lookup failed" (* error *)
+        end
+    | UnlockTVar (mk_tvar _ n k) =>
+        match lookup (k, n) m with
+        | Some (v, wv, l) =>
+          Ret (vc, add (k, n) (v, wv, false) m, tt)
+        | None => error "h_tl2 UnlockTVar lookup failed"
+        end
+    end.
+
+Definition handle_tvars {E} {K} (V : K -> Type) M
+  `{HMap (pkey K nat) (pkey_type V) M} `{Foldable M (sigT (@pkey_type K nat V))}:
+  tvarE V ~> stateT M (itree E) :=
+  fun _ t m =>
+    match t with
+    | NewTVar k v =>
+        let n := S (fold (fun '(existT _ (_, n) _) acc => max n acc) 0 m) in
+        Ret (add (k, n) v m, mk_tvar V n k)
+    | ReadTVar x =>
+        let '(mk_tvar _ n k) := x in
+        match lookup (k, n) m with
+        | Some v => Ret (m, v)
+        | None => ITree.spin (* error *)
+        end
+    | WriteTVar x v =>
+        (let '(mk_tvar _ n k) := x in
+         fun (v : V k) => Ret (add (k, n) v m, tt)) v
+    end.
+
+Definition h_tvars_tl2 {K} (V : K -> Type):
+  tvarE V ~> itree (tl2E V) :=
+  fun _ e =>
+    match e with
+    | NewTVar k v => ITree.trigger (NewTVarTL2 k v)
+    | ReadTVar x =>
+        '(v, _, _) <- trigger (ReadTVarTL2 x) ;;
+        Ret v
+    | WriteTVar x v => ITree.spin (* error *)
+    end.
+
+
+
+Section example.
+
+  #[global] Instance EqDec_unit : EqDec unit eq :=
+    fun x y => match x, y with tt, tt => left eq_refl end.
+
+  Definition nats (_ : unit) : Type := nat.
+
+  Definition fib_trans (x0 x1 : TVar nats nat): itree (stmE nats) unit :=
+    v0 <- readTVar x0 ;;
+    v1 <- readTVar x1 ;;
+    writeTVar x0 v1 ;;
+    writeTVar x1 (v0 + v1).
+
+  Definition fib (n : nat) : itree (runStmE nats +' forkE) unit :=
+    '(x, y) <- atomically (
+      x <- newTVar tt 0 ;;
+      y <- newTVar tt 1 ;;
+      Ret (x, y)) ;;
+    (fix fib_ n :=
+      match n with
+      | 0 => Ret tt
+      | S n => fork (atomically (fib_trans x y)) (fib_ n)
+      end) n.
+
+
+
+  Definition run_atomically {K} {V : K -> Type} {E A} (t0 : itree (runStmE V +' E) A):
+    itree (transactionE (stmE V) +' E) A :=
+    interp (bimap h_atomically (id_ _)) t0.
+
+  Definition run_atomic_transactions {K} `{EqDec K eq} {V : K -> Type}
+    (t1 : itree (transactionE (stmE V) +' forkE) unit):
+    itree void1 (halist (pkey K nat) (pkey_type V) * unit) :=
+    let t2 : itree (atomicE (tvarE V) +' forkE +' tvarE V) unit := translate (bimap atomic_transactions subevent) t1 in
+    let t3 : stateT _ _ _ := interp (handle_tvars _ _) (schedule_rr [t2]) in
+    t3 HMap.empty.
+
+
+
+  Definition h_trigger {E F} `{E -< F}: Handler E F :=
+    fun _ e => trigger e.
+
+  Definition run_single_lock {K} `{EqDec K eq} {V : K -> Type}
+    (t1 : itree (transactionE (stmE V) +' forkE) unit):
+    itree void1 (halist (pkey K nat) (pkey_type V) * (bool * unit)) :=
+    let t2 : itree (atomicE void1 +' forkE +' lockE +' tvarE V) unit :=
+      interp (case_ single_global_lock h_trigger) t1 in
+    let t3 := schedule_rr [t2] in
+    let t4 : stateT bool (itree (tvarE V)) unit := interp (case_ h_lock pure_state) t3 in
+    let t5 : stateT _ (itree void1) _ := interp (handle_tvars _ _) (t4 false) in
+    t5 HMap.empty.
+
+
+
+  Definition run_tl2 {K} `{EqDec K eq} {V : K -> Type}
+    (t1 : itree (transactionE (stmE V) +' forkE) unit)
+    : itree errorE (nat * halist (pkey K nat) (fun p => (V (fst p) * nat * bool)%type) * unit) :=
+    let t2 : itree (atomicE void1 +' forkE +' tl2E V +' errorE) unit :=
+      interp (case_ tl2 h_trigger) t1 in
+    let t3 : itree (tl2E V +' errorE) unit := schedule_rr [t2] in
+    let t4 : stateT _ (itree errorE) _ :=
+      interp (case_ (h_tl2 _) pure_state) t3 in
+    t4 (0, HMap.empty).
+
+
+
+  Variant result (E : Type -> Type) (A : Type) :=
+  | Val : A -> result E A
+  | NotYet : result E A
+  | Event : forall {X}, E X -> result E A.
+
+  Arguments Val {E A} (a).
+  Arguments NotYet {E A}.
+  Arguments Event {E A} {X} (e).
+
+  Definition force {E A} (n : nat) (t : itree E A) : result E A :=
+    match observe (burn n t) with
+    | RetF a => Val a
+    | TauF _ => NotYet
+    | VisF e _ => Event e
+    end.
+
+  Definition unwrap {E A} : option A -> itree E A :=
+    fun o => match o with None => ITree.spin | Some a => Ret a end.
+
+  Compute (force 178 (run_atomic_transactions (run_atomically (fib 8)))).
+  Compute (force 1000 (run_single_lock (run_atomically (fib 8)))).
+  Compute (force 1874 (run_tl2 (run_atomically (fib 8)))).
+
+  Definition read_test : itree (runStmE nats +' forkE) unit :=
+    x <- atomically (newTVar tt 21) ;;
+    atomically (readTVar x) ;;
+    Ret tt.
+
+  Definition write_test : itree (runStmE nats +' forkE) unit :=
+    x <- atomically (newTVar tt 22) ;;
+    atomically (writeTVar x 23).
+
+  Definition inc_test : itree (runStmE nats +' forkE) unit :=
+    x <- atomically (newTVar tt 0) ;;
+    atomically (v <- readTVar x ;; writeTVar x (S v)).
+
+  Compute (force 1000 (run_tl2 (run_atomically read_test))).
+  Compute (force 1000 (run_tl2 (run_atomically write_test))).
+  Compute (force 1000 (run_tl2 (run_atomically inc_test))).
+
+  Definition takeMVar {K} {V : K -> Type} {A} (t : TVar V (option A)) : itree (stmE V) A :=
+    v <- readTVar t ;;
+    match v with
+    | None => retry
+    | Some a => writeTVar t None ;; Ret a
+    end.
+
+  Definition putMVar {K} {V : K -> Type} {A} (t : TVar V (option A)) (a : A) : itree (stmE V) unit :=
+    v <- readTVar t ;;
+    match v with
+    | None => writeTVar t (Some a)
+    | Some _ => retry
+    end.
+
+  Inductive Ty :=
+  | Nat : Ty
+  | Opt : Ty -> Ty.
+
+  Definition Ty_dec (x y : Ty) : {x = y} + {x <> y}.
+    decide equality.
+  Defined.
+
+  #[global] Instance EqDec_Types : EqDec Ty eq := Ty_dec.
+
+  Fixpoint D (type : Ty) : Type :=
+    match type with
+    | Nat => nat
+    | Opt t => option (D t)
+    end.
+
+  Definition message_passing : itree (runStmE D +' forkE) unit :=
+    mv <- atomically (newTVar (Opt Nat) None) ;;
+    done <- atomically (newTVar Nat 0) ;;
+    fork (v1 <- atomically (takeMVar mv) ;; v2 <- atomically (takeMVar mv) ;; atomically (putMVar mv (v1 + v2)))
+         (atomically (putMVar mv 3) ;; atomically (putMVar mv 4) ;; atomically (V := D) (r <- takeMVar mv ;; writeTVar done r)).
+
+  Definition message_passing_simple : itree (runStmE D +' forkE) unit :=
+    mv <- atomically (newTVar (Opt Nat) None) ;;
+    done <- atomically (newTVar Nat 0) ;;
+    fork (v1 <- atomically (takeMVar mv) ;; atomically (putMVar mv (v1 * v1)))
+         (atomically (putMVar mv 3) ;; atomically (V := D) (r <- takeMVar mv ;; writeTVar done r)).
+
+  Definition message_passing_simpler : itree (runStmE D +' forkE) unit :=
+    mv <- atomically (newTVar (Opt Nat) None) ;;
+    done <- atomically (newTVar Nat 0) ;;
+    fork (v1 <- atomically (takeMVar mv) ;; atomically (writeTVar done (v1 * v1)))
+         (atomically (putMVar mv 3)).
+
+  Compute (force 100 (run_atomic_transactions (run_atomically message_passing_simpler))).
+  Compute (force 100 (run_atomic_transactions (run_atomically message_passing_simple))).
+  Compute (force 100 (run_atomic_transactions (run_atomically message_passing))).
+  Compute (force 200 (run_single_lock (run_atomically message_passing_simpler))).
+  Compute (force 200 (run_single_lock (run_atomically message_passing_simple))).
+  Compute (force 300 (run_single_lock (run_atomically message_passing))).
+  Compute (force 1000 (run_tl2 (run_atomically message_passing_simpler))).
+  Compute (force 1000 (run_tl2 (run_atomically message_passing_simple))).
+  Compute (force 1000 (run_tl2 (run_atomically message_passing))).
+
+  (* TODO: tests with orElse *)
+
+End example.
+
+
+
