theories/Monads/STM/Schedule.v
@@ -1,0 +1,34 @@
+From Crane Require Import Monads.ITree.
+
+From Stdlib Require Import Arith.PeanoNat List.
+
+Import ListNotations.
+
+From ITree Require Import Basics.Basics.
+
+Open Scope itree_scope.
+
+(* Scheduler implementations should be such that 0 getting chosen infinitely often will ensure that every thread gets scheduled *)
+Variant scheduleE : Type -> Type :=
+| Schedule (n : nat) : scheduleE {m : nat | m < n}.
+
+Definition h_rr {E} : scheduleE ~> itree E :=
+  fun _ e =>
+    match e with
+    | Schedule n =>
+        match n with
+        | 0 => ITree.spin (* error *)
+        | S m => Ret (exist _ 0 (PeanoNat.Nat.lt_0_succ m))
+        end
+    end.
+
+Fixpoint signth {A} (l : list A) (n : {m : nat | m < length l}) : A :=
+  match l, n with
+  | [], exist _ m H => False_rect _ (PeanoNat.Nat.nlt_0_r m H)
+  | (v :: l), exist _ m H =>
+    match m with
+    | 0 => fun _ => v
+    | S m => fun H : S m < S (length l) => signth l (exist _ m (PeanoNat.lt_S_n _ _ H))
+    end H
+  end.
+
